progress on valid_interleave semantics

legion.v
@@ -90,14 +90,16 @@ with list_T : Set :=
  | Nil_list_T : list_T
  | Cons_list_T (_:T) (_:list_T).
 
-Inductive Clobber : Set := 
- | S_Null : Clobber.
 
 Inductive H : Set := 
  | H_Hl (H5:H) (l5:l).
 
 Inductive id : Set := 
 .
+Inductive privs : Set := 
+| priv_excl
+| priv_atomic.
+
 
 Inductive ee : Set := 
  | ee_Elist (_:list_e)
@@ -137,28 +139,26 @@ with e : Set :=
  | E_True : e (*r constant true *)
  | E_False : e (*r constant false *)
  | E_Zero : e
- | E_Succ (Clobber5:Clobber) (iv5:iv)
+ | E_Succ (Clobber5:list emem) (iv5:iv)
 with list_e : Set := 
  | Nil_list_e : list_e
  | Cons_list_e (_:e) (_:list_e)
 with list_id_rr_ee : Set := 
  | Nil_list_id_rr_ee : list_id_rr_ee
- | Cons_list_id_rr_ee (_:id) (_:rr) (_:ee) (_:list_id_rr_ee).
+ | Cons_list_id_rr_ee (_:id) (_:rr) (_:ee) (_:list_id_rr_ee)
+with emem : Set := 
+ | em_ReadE (e1:e) (privs5:privs) (e2:e) (e3:e)
+ | em_WriteE (e1:e) (privs5:privs) (e2:e) (e3:e)
+ | em_ReduceIdE (e1:e) (privs5:privs) (e2:e) (e3:e).
 
-Inductive excl : Set := 
-| EX_Nil
-| EX_NotNil.
-
-Inductive emem : Set := 
- | em_ReadE (e1:e) (excl5:excl) (e2:e) (e3:e)
- | em_WriteE (e1:e) (excl5:excl) (e2:e) (e3:e)
- | em_ReduceIdE (e1:e) (excl5:excl) (e2:e) (e3:e).
 
 Inductive om : Set := 
  | o_Subregion (r1:r) (r2:r)
  | o_Disjointness (r1:r) (r2:r).
 
 Definition E := (list emem) % type.
+
+Definition Clobber : (list emem) % type.
 
 (* | [] : E
  | E_Append (E5:E) (emem5:emem). *)
@@ -610,84 +610,6 @@ Fixpoint app_list_r (l0 m: list_r): list_r :=
   end.
 
 
-(* FIXME: make this type correctly *)
-Definition IntOp (_ _:e) := E_PlaceHolder.
-Definition Comp (_ _:e) := E_PlaceHolder.
-
-(* how to do the substitution? *)
-Fixpoint apply_mem (S:Clobber) (E : E) :=
-match S, E with
-| S', [] => S'
-| S', (em_ReadE _ _ _ _)::E' => apply_mem S' E'
-| S', (em_WriteE l _ v _)::E' => (apply_mem S' E')  (* [v/l] *)
-| S', (em_ReduceIdE l _ v _)::E' => let S' := apply_mem S E' in
-                                    S' (* S'[id(S'(l),v)/l]  *)
-end.
-
-Fixpoint coherent (S:Clobber) (L1:list emem) (L2:list emem) E :=
-  match S, L1, L2, E with
-| S', L1', L2', [] => True
-| S', L1', L2', eps :: E' =>
-  match eps with
-  | em_ReadE l c v t => 
-    (* In l L2 -> *) coherent S' L1' L2' E'
-  | em_WriteE l c v t =>
-    ( (* In l L1 -> *) coherent (apply_mem S' [eps]) L1' (* (l:: *) (L2') E') \/
-    coherent (apply_mem S' [eps]) L1' L2' E'
-  | _ =>
-    coherent (apply_mem S' [eps]) L1' L2' E'
-  end
-end.
-
-Fixpoint any_interleave (l:list E) :=
-  if fold_right (fun a b => andb
-                              (match a with
-                               | [] => true
-                               | _ => false
-                               end)
-                                 b) true l then
-    True
-  else (* take an item off the front of the list *)
-    False.
-
-Fixpoint Lexcl E (C:Clobber) :=
-  filter (fun a =>
-            match a with
-            | em_ReadE l EX_Nil v t => true
-            | em_WriteE l EX_Nil  v t => true
-            | em_ReduceIdE l EX_Nil v t => true
-            | _ => false 
-            end) E.
-
-Fixpoint Latomic E (C:Clobber) :=
-  filter (fun a =>
-            match a with
-            | em_ReadE l EX_NotNil v t => true
-            | em_WriteE l EX_NotNil  v t => true
-            | em_ReduceIdE l EX_NotNil v t => true
-            | _ => false 
-            end) E.
-
-Fixpoint seq_equiv S L1 L2 E' (l: list E) :=
-  coherent S L1 L2 (fold_right (fun a b => a ++ b) [] l) /\
-  forall l, apply_mem S E'  = apply_mem S (fold_right (fun a b => a ++ b) [] l).
-
-Fixpoint valid_interleave S C (E':E) (l: list E) :=
-  any_interleave ([E']++l) /\
-  coherent S (Lexcl E' C) (Lexcl E' C) E' /\
-  seq_equiv S (Lexcl  E' C) (Lexcl E' C) E' l (* /\
-  forall t, S (Latomic E' C) nil E' (* fold append here *) *)
-.
-(* what is mark coherence doing here? *)
-
-Fixpoint mark_coherence l (Q:Q) (taskid:nat):excl :=
-match l,Q with
-| [],Q' => EX_Nil
-| em_ReadE l c v t :: E', Q' => EX_NotNil
-| em_WriteE l c v t :: E', Q' => EX_NotNil
-| em_ReduceIdE l c v t :: E', Q'  => EX_NotNil
-end.
-
 (** subrules *)
 Fixpoint is_v_of_rho_list (l:list_rho) : Prop :=
   match l with
@@ -826,9 +748,9 @@ end.
 
 Definition is_emem_of_emem (emem5:emem) : Prop :=
   match emem5 with
-  | (em_ReadE e1 excl5 e2 e3) => ((is_e_of_e e1) /\ (is_e_of_e e2) /\ (is_e_of_e e3))
-  | (em_WriteE e1 excl5 e2 e3) => ((is_e_of_e e1) /\ (is_e_of_e e2) /\ (is_e_of_e e3))
-  | (em_ReduceIdE e1 excl5 e2 e3) => ((is_e_of_e e1) /\ (is_e_of_e e2) /\ (is_e_of_e e3))
+  | (em_ReadE e1 privs5 e2 e3) => ((is_e_of_e e1) /\ (is_e_of_e e2) /\ (is_e_of_e e3))
+  | (em_WriteE e1 privs5 e2 e3) => ((is_e_of_e e1) /\ (is_e_of_e e2) /\ (is_e_of_e e3))
+  | (em_ReduceIdE e1 privs5 e2 e3) => ((is_e_of_e e1) /\ (is_e_of_e e2) /\ (is_e_of_e e3))
 end.
 
 Fixpoint is_L_of_L (L_6:L) : Prop :=
@@ -954,11 +876,6 @@ Proof.
 Defined.
 Hint Resolve eq_H : ott_coq_equality.
 
-Lemma eq_Clobber: forall (x y : Clobber), {x = y} + {x <> y}.
-Proof.
-  decide equality; auto with ott_coq_equality arith.
-Defined.
-Hint Resolve eq_Clobber : ott_coq_equality.
 
 Lemma eq_bv: forall (x y : bv), {x = y} + {x <> y}.
 Proof.
@@ -1002,11 +919,11 @@ Hint Resolve eq_list_T : ott_coq_equality.
 
 
 
-Lemma eq_excl: forall (x y : excl), {x = y} + {x <> y}.
+Lemma eq_privs: forall (x y : privs), {x = y} + {x <> y}.
 Proof.
   decide equality; auto with ott_coq_equality arith.
 Defined.
-Hint Resolve eq_excl : ott_coq_equality.
+Hint Resolve eq_privs : ott_coq_equality.
 
 Lemma eq_rho: forall (x y : rho), {x = y} + {x <> y}.
 Proof.
@@ -1022,8 +939,12 @@ Hint Resolve eq_list_rho : ott_coq_equality.
 
 Fixpoint eq_e (x y : e): {x = y} + {x <> y} 
 with eq_list_e (x y : list_e): {x = y} + {x <> y}
-with eq_ee (x y : ee): {x = y} + {x <> y}.
+with eq_ee (x y : ee): {x = y} + {x <> y}
+with eq_emem (x y : emem): {x = y} + {x <> y}.
 Proof.
+
+  decide equality; auto with ott_coq_equality arith.
+  decide equality; auto with ott_coq_equality arith.
   decide equality; auto with ott_coq_equality arith.
   decide equality; auto with ott_coq_equality arith.
   decide equality; auto with ott_coq_equality arith.
@@ -1032,6 +953,7 @@ Defined.
 Hint Resolve eq_e : ott_coq_equality.
 Hint Resolve eq_list_e : ott_coq_equality.
 Hint Resolve eq_ee : ott_coq_equality.
+Hint Resolve eq_emem : ott_coq_equality.
 
 Lemma eq_list_e_T: forall (x y : list_e_T), {x = y} + {x <> y}.
 Proof.
@@ -1056,13 +978,6 @@ Proof.
   decide equality; auto with ott_coq_equality arith.
 Defined.
 Hint Resolve eq_L : ott_coq_equality.
-
-Lemma eq_emem: forall (x y : emem), {x = y} + {x <> y}.
-Proof.
-  decide equality; auto with ott_coq_equality arith.
-Defined.
-Hint Resolve eq_emem : ott_coq_equality.
-
 
 Lemma eq_E: forall (x y : E), {x = y} + {x <> y}.
 Proof.
@@ -1113,6 +1028,148 @@ Fixpoint app_list_id (l0 m: list_id): list_id :=
   end.
 
 (** definitions *)
+(* FIXME: make this type correctly *)
+Definition IntOp (_ _:e) := E_PlaceHolder.
+Definition Comp (_ _:e) := E_PlaceHolder.
+
+(* how to do the substitution? *)
+Fixpoint apply_mem (S:list emem) (E : E) :=
+match S, E with
+| S', [] => S'
+| S', (em_ReadE _ _ _ _)::E' => apply_mem S' E'
+| S', (em_WriteE l _ v _)::E' => (apply_mem S' E')  (* [v/l] *)
+| S', (em_ReduceIdE l _ v _)::E' => let S' := apply_mem S E' in
+                                    S' (* S'[id(S'(l),v)/l]  *)
+end.
+
+Fixpoint coherent (S:list emem) (L1:list emem) (L2:list emem) (E: list emem) :=
+  match S, L1, L2, E with
+| S', L1', L2', [] => True
+| S', L1', L2', eps :: E' =>
+  match eps with
+  | em_ReadE l c v t => 
+    (* In l L2 -> *) coherent S' L1' L2' E'
+  | em_WriteE l c v t =>
+    ( (* In l L1 -> *) coherent (apply_mem S' [eps]) L1' (* (l:: *) (L2') E') \/
+    coherent (apply_mem S' [eps]) L1' L2' E'
+  | _ =>
+    coherent (apply_mem S' [eps]) L1' L2' E'
+  end
+end.
+
+(* think you need an accumulator here
+one of the things you have to do is take an element off until you reach the end of it.
+
+
+ *)
+
+(* remainder list, implemented separately to shut up Coq's termination checker *)
+
+Fixpoint rem_list m (acc: list (list emem)) (l: list (list emem)) :=
+  match l with
+  | [] => []
+  | E :: l' =>
+    match E with
+    | [] => rem_list m (acc++[[]]) l'
+    | a :: E' =>
+      if eq_emem m a then
+        acc ++ [E'] ++ l'
+      else
+        rem_list m (acc ++ [E]) l'
+    end
+  end.
+
+Fixpoint any_interleave (E:list emem) (l:list (list emem)) :=
+  match E with
+  | [] =>
+    if fold_right (fun a b => andb
+                              (match a with
+                               | [] => true
+                               | _ => false
+                               end)
+                                 b) true l then
+      True
+    else
+      False
+  | a :: l' =>
+    any_interleave l' (rem_list a [] l)
+    (* need a list with a front and back
+       so you need an accumulator.
+     *)
+  end.
+
+Fixpoint member m l :=
+  match l with
+  | [] => false
+  | m' :: l' =>
+    if eq_emem m m' then
+      true
+    else
+      member m l'
+  end.
+
+Fixpoint Lexcl E (C:list emem) :=
+  filter (fun x => negb (member x C))
+         (filter (fun a =>
+            match a with
+            | em_ReadE l priv_excl v t => true
+            | em_WriteE l priv_excl  v t => true
+            | em_ReduceIdE l priv_excl v t => true
+            | _ => false 
+            end) E).
+
+Fixpoint Latomic E (C:list emem) :=
+  filter (fun x => negb (member x (C++(Lexcl E C))))
+         (filter (fun a =>
+            match a with
+            | em_ReadE l priv_atomic v t => true
+            | em_WriteE l priv_atomic  v t => true
+            | em_ReduceIdE l priv_atomic v t => true
+            | _ => false 
+            end) E).
+
+Fixpoint seq_equiv S L1 L2 (E':E) (l: list E) :=
+  coherent S L1 L2 (fold_right (fun a b => a ++ b) [] l) /\
+  forall l, apply_mem S E'  = apply_mem S (fold_right (fun a b => a ++ b) [] l).
+
+Fixpoint down_t (t:e) (E: list emem) :=
+  match E with
+  | [] => []
+  | em_ReadE l c v t' :: E' =>
+    if eq_e t t' then
+      (em_ReadE l c v t') :: down_t t E'
+    else
+      E'
+  | em_WriteE l c  v t' :: E' => 
+    if eq_e t t' then
+      (em_WriteE l c v t') :: down_t t E'
+    else
+      E'
+  | em_ReduceIdE l c v t' :: E' =>
+    if eq_e t t' then
+      (em_ReduceIdE l c v t') :: down_t t E'
+    else
+      E'
+  end.
+
+Fixpoint valid_interleave S C (E':E) (l: list E) :=
+  any_interleave ([E']++l) /\
+  coherent S (Lprivs E' C) (Lprivs E' C) E' /\
+  seq_equiv S (Lprivs  E' C) (Lprivs E' C) E' l /\ 
+  forall t, seq_equiv S (Latomic E' C) nil (down_t t E') [(down_t t (fold_right (fun a b => a ++ b) [] l))].
+
+(* fold append here *)
+
+(* what is mark coherence doing here? *)
+
+Fixpoint mark_coherence l (Q:Q) (taskid:nat):privs :=
+match l,Q with
+| [],Q' => priv_excl
+| em_ReadE l c v t :: E', Q' => priv_atomic
+| em_WriteE l c v t :: E', Q' => priv_atomic
+| em_ReduceIdE l c v t :: E', Q'  => priv_atomic
+end.
+
 
 (* defns Jtype *)
 Inductive typing : G -> P -> Omega -> e -> T -> Prop :=    (* defn typing *)
@@ -1196,12 +1253,12 @@ is_G_of_G G5 ->
 (** definitions *)
 
 (* defns Jop *)
-Inductive eval : M -> L -> H -> Clobber -> list e -> e -> e -> E -> Prop :=    (* defn eval *)
- | EVa : forall (M5:M) (L5:L) (H5:H) (Clobber5:Clobber) (C5:list e) (x:termvar) (v5:e) (E5:E),
+Inductive eval : M -> L -> H -> list emem -> list e -> e -> e -> E -> Prop :=    (* defn eval *)
+ | EVa : forall (M5:M) (L5:L) (H5:H) (Clobber5:list emem) (C5:list e) (x:termvar) (v5:e) (E5:E),
      is_L_of_L L5 ->
      is_v_of_e v5 ->
      eval M5 L5 H5 Clobber5 C5 (E_Va x) v5 E5
- | ERead1 : forall (M5:M) (L5:L) (H5:H) (Clobber5:Clobber) (C5:list e) (e5:e) (E5:E) (l5:l) (excl5:excl) (v5:e) (Clobber':Clobber)
+ | ERead1 : forall (M5:M) (L5:L) (H5:H) (Clobber5:list emem) (C5:list e) (e5:e) (E5:E) (l5:l) (privs5:privs) (v5:e) (Clobber':list emem)
      (prodvalue: eval M5 L5 H5 Clobber5 C5 e5 (E_MemoryLoc l5) E5)
      (apply:   Clobber'   =   (apply_mem Clobber5 E5)  )
      (memnotclobber:  (not (   In   (E_MemoryLoc l5)     C5    )) ),
@@ -1209,25 +1266,26 @@ Inductive eval : M -> L -> H -> Clobber -> list e -> e -> e -> E -> Prop :=    (
      is_e_of_e e5 ->
      is_v_of_e v5 ->
      is_v_of_e v5 ->
-     eval M5 L5 H5 Clobber5 C5 (E_Read e5) v5  ( E5  ++ [em_ReadE (E_MemoryLoc l5) excl5 v5 E_Zero] ) 
- | ERead2 : forall (M5:M) (L5:L) (H5:H) (Clobber5:Clobber) (C5:list e) (e5:e) (l5:l) (E5:E) (excl5:excl) (v5:e) (Clobber':Clobber)
+     eval M5 L5 H5 Clobber5 C5 (E_Read e5) v5  ( E5  ++ [em_ReadE (E_MemoryLoc l5) privs5 v5 E_Zero] ) 
+ | ERead2 : forall (M5:M) (L5:L) (H5:H) (Clobber5:list emem) (C5:list e) (e5:e) (l5:l) (E5:E) (privs5:privs) (v5:e) (Clobber':list emem)
      (prodvalue: eval M5 L5 H5 Clobber5 C5 e5 (E_MemoryLoc l5) E5)
      (apply:   Clobber'   =   (apply_mem Clobber5 E5)  )
      (memclobber:  In   (E_MemoryLoc l5)  C5  ),
      is_L_of_L L5 ->
      is_e_of_e e5 ->
      is_v_of_e v5 ->
-     eval M5 L5 H5 Clobber5 C5 (E_Read e5) (E_HeapVal (H_Hl H5 l5))  ( E5 ++ [em_ReadE (E_MemoryLoc l5) excl5 v5 E_Zero] ) 
- | EWrite : forall (M5:M) (L5:L) (H5:H) (Clobber5:Clobber) (C5:list e) (e1 e2:e) (l5:l) (E_5 E1:E) (Clobber':Clobber) (v5:e) (E2:E)
+     eval M5 L5 H5 Clobber5 C5 (E_Read e5) (E_HeapVal (H_Hl H5 l5))  ( E5 ++ [em_ReadE (E_MemoryLoc l5) privs5 v5 E_Zero] ) 
+ | EWrite : forall (M5:M) (L5:L) (H5:H) (Clobber5:list emem) (C5:list e) (e1 e2:e) (l5:l) (E_5 E1:E) (Clobber':list emem) (v5:e) (E2:E)
      (prod1value: eval M5 L5 H5 Clobber5 C5 e1 (E_MemoryLoc l5) E1)
      (prod2value: eval M5 L5 H5 Clobber' C5 e2 v5 E2)
+     (validinterleave: valid_interleave Clobber5 Clobber' E_5 ([E1]++[E2])) 
      (apply:   Clobber'   =   (apply_mem Clobber5 E_5)  ) ,
      is_L_of_L L5 ->
      is_e_of_e e1 ->
      is_e_of_e e2 ->
      is_v_of_e v5 ->
      eval M5 L5 H5 Clobber5 C5 (E_Write e1 e2) (E_MemoryLoc l5) E_5
- | EReduce : forall (M5:M) (L5:L) (H5:H) (Clobber5:Clobber) (C5:list e) (id5:id) (e1 e2:e) (l5:l) (E_5 E1:E) (Clobber':Clobber) (v5:e) (E2:E)
+ | EReduce : forall (M5:M) (L5:L) (H5:H) (Clobber5:list emem) (C5:list e) (id5:id) (e1 e2:e) (l5:l) (E_5 E1:E) (Clobber':list emem) (v5:e) (E2:E)
      (prod1value: eval M5 L5 H5 Clobber5 C5 e1 (E_MemoryLoc l5) E1)
      (prod2value: eval M5 L5 H5 Clobber' C5 e2 v5 E2),
      is_L_of_L L5 ->
@@ -1235,7 +1293,7 @@ Inductive eval : M -> L -> H -> Clobber -> list e -> e -> e -> E -> Prop :=    (
      is_e_of_e e2 ->
      is_v_of_e v5 ->
      eval M5 L5 H5 Clobber5 C5 (E_Reduce id5 e1 e2) (E_MemoryLoc l5) E_5
- | EReduceId : forall (M5:M) (L5:L) (H5:H) (Clobber5:Clobber) (C5:list e) (l5:l) (e1 e2 e3 v_5:e) (E_5:E) (v1:e) (E1:E) (Clobber':Clobber) (v2:e) (E2:E) (v3:e) (E3:E) (v4:e)
+ | EReduceId : forall (M5:M) (L5:L) (H5:H) (Clobber5:list emem) (C5:list e) (l5:l) (e1 e2 e3 v_5:e) (E_5:E) (v1:e) (E1:E) (Clobber':list emem) (v2:e) (E2:E) (v3:e) (E3:E) (v4:e)
      (prod1value: eval M5 L5 H5 Clobber5 C5 (E_MemoryLoc l5) v1 E1)
      (prod2value: eval M5 L5 H5 Clobber' C5 e1 v2 E2)
      (prod3value: eval M5 L5 H5 Clobber' C5 e2 v3 E3)
@@ -1250,50 +1308,50 @@ Inductive eval : M -> L -> H -> Clobber -> list e -> e -> e -> E -> Prop :=    (
      is_v_of_e v3 ->
      is_v_of_e v4 ->
      eval M5 L5 H5 Clobber5 C5 (E_Reduceid l5 e1 e2 e3) v_5 E_5
- | ENull : forall (M5:M) (L5:L) (H5:H) (Clobber5:Clobber) (C5:list e),
+ | ENull : forall (M5:M) (L5:L) (H5:H) (Clobber5:list emem) (C5:list e),
      is_L_of_L L5 ->
      eval M5 L5 H5 Clobber5 C5 E_NullLoc E_NullLoc []
- | ENew : forall (M5:M) (L5:L) (H5:H) (Clobber5:Clobber) (C5:list e) (T5:T) (r5:r) (l5:l),
+ | ENew : forall (M5:M) (L5:L) (H5:H) (Clobber5:list emem) (C5:list e) (T5:T) (r5:r) (l5:l),
      is_L_of_L L5 ->
      eval M5 L5 H5 Clobber5 C5 (E_New T5 r5) (E_MemoryLoc l5) []
- | ENullTrue : forall (M5:M) (L5:L) (H5:H) (Clobber5:Clobber) (C5:list e) (T5:T),
+ | ENullTrue : forall (M5:M) (L5:L) (H5:H) (Clobber5:list emem) (C5:list e) (T5:T),
      is_L_of_L L5 ->
      eval M5 L5 H5 Clobber5 C5 (E_NullFn T5 r_Null) (E_Base1 bv_True) []
- | ENullFalse : forall (M5:M) (L5:L) (H5:H) (Clobber5:Clobber) (C5:list e) (T5:T) (r5:r),
+ | ENullFalse : forall (M5:M) (L5:L) (H5:H) (Clobber5:list emem) (C5:list e) (T5:T) (r5:r),
      is_L_of_L L5 ->
       (not (    (T_PointerOne T5 r5)   =   (T_PointerOne T5 r_Null)    ))  ->
      eval M5 L5 H5 Clobber5 C5 (E_NullFn T5 r5) (E_Base1 bv_False) []
- | EIsNullTrue : forall (M5:M) (L5:L) (H5:H) (Clobber5:Clobber) (C5:list e) (l5:l) (e1:e) (E1:E)
+ | EIsNullTrue : forall (M5:M) (L5:L) (H5:H) (Clobber5:list emem) (C5:list e) (l5:l) (e1:e) (E1:E)
      (prod1value: eval M5 L5 H5 Clobber5 C5 e1 (E_MemoryLoc l5) E1),
      is_L_of_L L5 ->
      is_e_of_e e1 ->
        (E_MemoryLoc l5)   =   E_NullLoc   ->
      eval M5 L5 H5 Clobber5 C5 (E_isNull (E_MemoryLoc l5)) (E_Base1 bv_True) []
- | EIsNullFalse : forall (M5:M) (L5:L) (H5:H) (Clobber5:Clobber) (C5:list e) (l5:l) (e1:e) (E1:E)
+ | EIsNullFalse : forall (M5:M) (L5:L) (H5:H) (Clobber5:list emem) (C5:list e) (l5:l) (e1:e) (E1:E)
      (prod1value: eval M5 L5 H5 Clobber5 C5 e1 (E_MemoryLoc l5) E1),
      is_L_of_L L5 ->
      is_e_of_e e1 ->
       (not (    (E_MemoryLoc l5)   =   E_NullLoc    ))  ->
      eval M5 L5 H5 Clobber5 C5 (E_isNull (E_MemoryLoc l5)) (E_Base1 bv_False) []
- | EUpRgn : forall (r_list:list_r) (M5:M) (L5:L) (H5:H) (Clobber5:Clobber) (C5:list e) (e5 v5:e) (E5:E)
+ | EUpRgn : forall (r_list:list_r) (M5:M) (L5:L) (H5:H) (Clobber5:list emem) (C5:list e) (e5 v5:e) (E5:E)
      (prodvalue: eval M5 L5 H5 Clobber5 C5 e5 v5 E5),
      is_L_of_L L5 ->
      is_e_of_e e5 ->
      is_v_of_e v5 ->
      eval M5 L5 H5 Clobber5 C5 (E_UpRegion e5 r_list) v5 E5
- | EDnRgn1 : forall (r_list:list_r) (M5:M) (L5:L) (H5:H) (Clobber5:Clobber) (C5:list e) (e5:e) (l5:l) (E5:E) (v5:e)
+ | EDnRgn1 : forall (r_list:list_r) (M5:M) (L5:L) (H5:H) (Clobber5:list emem) (C5:list e) (e5:e) (l5:l) (E5:E) (v5:e)
      (prodvalue: eval M5 L5 H5 Clobber5 C5 e5 v5 E5),
      is_L_of_L L5 ->
      is_e_of_e e5 ->
      is_v_of_e v5 ->
      eval M5 L5 H5 Clobber5 C5 (E_DownRegion e5 r_list) (E_MemoryLoc l5) E5
- | EDnRgn2 : forall (r_list:list_r) (M5:M) (L5:L) (H5:H) (Clobber5:Clobber) (C5:list e) (e5:e) (E5:E) (v5:e)
+ | EDnRgn2 : forall (r_list:list_r) (M5:M) (L5:L) (H5:H) (Clobber5:list emem) (C5:list e) (e5:e) (E5:E) (v5:e)
      (prodvalue: eval M5 L5 H5 Clobber5 C5 e5 v5 E5),
      is_L_of_L L5 ->
      is_e_of_e e5 ->
      is_v_of_e v5 ->
      eval M5 L5 H5 Clobber5 C5 (E_DownRegion e5 r_list) E_NullLoc E5
- | EColor : forall (M5:M) (L5:L) (H5:H) (Clobber5:Clobber) (C5:list e) (e1 e2 e3:e) (K':K) (E':E) (l5:l) (E1:E) (Clobber':Clobber) (v5:e) (E2:E) (Clobber'':Clobber) (E3:E)
+ | EColor : forall (M5:M) (L5:L) (H5:H) (Clobber5:list emem) (C5:list e) (e1 e2 e3:e) (K':K) (E':E) (l5:l) (E1:E) (Clobber':list emem) (v5:e) (E2:E) (Clobber'':list emem) (E3:E)
      (prod1value: eval M5 L5 H5 Clobber5 C5 e1 (E_MemoryLoc l5) E1)
      (prod2value: eval M5 L5 H5 Clobber' C5 e2 v5 E2)
      (prod3value: eval M5 L5 H5 Clobber'' C5 e3 v5 E3),
@@ -1303,10 +1361,10 @@ Inductive eval : M -> L -> H -> Clobber -> list e -> e -> e -> E -> Prop :=    (
      is_e_of_e e3 ->
      is_v_of_e v5 ->
      eval M5 L5 H5 Clobber5 C5 (E_Color e1 e2 e3) (E_Kthing K') E'
- | ENewColor : forall (M5:M) (L5:L) (H5:H) (Clobber5:Clobber) (C5:list e) (r5:r) (K5:K),
+ | ENewColor : forall (M5:M) (L5:L) (H5:H) (Clobber5:list emem) (C5:list e) (r5:r) (K5:K),
      is_L_of_L L5 ->
      eval M5 L5 H5 Clobber5 C5 (E_NewColor r5) (E_Kthing K5) []
- | EPartition : forall (r_list:list_r) (p:index) (M5:M) (L5:L) (H5:H) (Clobber5:Clobber) (C5:list e) (e1 e2:e) (l5:l) (E':E) (K5:K) (E1:E) (Clobber':Clobber) (v5:e) (E2:E) (t105:r)
+ | EPartition : forall (r_list:list_r) (p:index) (M5:M) (L5:L) (H5:H) (Clobber5:list emem) (C5:list e) (e1 e2:e) (l5:l) (E':E) (K5:K) (E1:E) (Clobber':list emem) (v5:e) (E2:E) (t105:r)
      (prod1value: eval M5 L5 H5 Clobber5 C5 e1 (E_Kthing K5) E1)
      (prod2value: eval M5 L5 H5 Clobber' C5 e2 v5 E2),
           nth_list_r (p - 1) r_list = Some t105 ->
@@ -1315,13 +1373,13 @@ is_L_of_L L5 ->
      is_e_of_e e2 ->
      is_v_of_e v5 ->
      eval M5 L5 H5 Clobber5 C5 (E_Part t105 e1 r_list e2) (E_MemoryLoc l5) E'
- | EPack : forall (M5:M) (L5:L) (H5:H) (Clobber5:Clobber) (C5:list e) (e1:e) (T1:T) (v':e) (E_5:E) (K5:K) (E1:E)
+ | EPack : forall (M5:M) (L5:L) (H5:H) (Clobber5:list emem) (C5:list e) (e1:e) (T1:T) (v':e) (E_5:E) (K5:K) (E1:E)
      (prod1value: eval M5 L5 H5 Clobber5 C5 e1 (E_Kthing K5) E1),
      is_L_of_L L5 ->
      is_e_of_e e1 ->
      is_v_of_e v' ->
      eval M5 L5 H5 Clobber5 C5 (E_Pack e1 T1) v' E_5
- | EUnpack : forall (rho_list:list_rho) (M5:M) (L5:L) (H5:H) (Clobber5:Clobber) (C5:list e) (e1:e) (id5:id) (T1:T) (e2 v2:e) (E':E) (v_5:e) (E1:E) (L':L) (v1:e) (M':M) (Clobber':Clobber) (E2:E)
+ | EUnpack : forall (rho_list:list_rho) (M5:M) (L5:L) (H5:H) (Clobber5:list emem) (C5:list e) (e1:e) (id5:id) (T1:T) (e2 v2:e) (E':E) (v_5:e) (E1:E) (L':L) (v1:e) (M':M) (Clobber':list emem) (E2:E)
      (prod1memval: eval M5 L5 H5 Clobber5 C5 e1 (E_RegRelInst rho_list v_5) E1)
      (lreplace:   L'   =   (L_LRepl L5 v1 id5)  )
      (prod2value: eval M' L' H5 Clobber' C5 e2 v_5 E2),
@@ -1333,7 +1391,7 @@ is_L_of_L L5 ->
      is_L_of_L L' ->
      is_v_of_e v1 ->
      eval M5 L5 H5 Clobber5 C5 (E_Unpack e1 id5 T1 e2) v2 E'
- | ECall : forall (e_v_list:list_e_e) (r_list:list_r) (n:index) (M5:M) (L5:L) (H5:H) (Clobber5:Clobber) (C5:list e) (id5:id) (E'':E) (L':L) (t106:(e*e))
+ | ECall : forall (e_v_list:list_e_e) (r_list:list_r) (n:index) (M5:M) (L5:L) (H5:H) (Clobber5:list emem) (C5:list e) (id5:id) (E'':E) (L':L) (t106:(e*e))
      (memreplace:   L'   =   (L_LMapping L5 e_v_list)  ),
           nth_list_e_e (n - 1) e_v_list = Some t106 ->
 is_L_of_L L5 ->
@@ -1341,7 +1399,7 @@ is_L_of_L L5 ->
      (Forall (fun (tmp_:(e*e)) => match tmp_ with (e_,v_) => is_e_of_e e_ end) (unmake_list_e_e e_v_list)) ->
      (Forall (fun (tmp_:(e*e)) => match tmp_ with (e_,v_) => is_v_of_e v_ end) (unmake_list_e_e e_v_list)) ->
      eval M5 L5 H5 Clobber5 C5 (E_FuncCall id5 r_list (make_list_e (map_list_e_e (fun (e_:e) (v_:e) => e_) e_v_list))) (match t106 with (e_,v_) => v_ end) E''
- | EIntOp : forall (M5:M) (L5:L) (H5:H) (Clobber5:Clobber) (C5:list e) (e1 e2 v_5:e) (E_5:E) (v1:e) (E1:E) (v2:e) (E2:E)
+ | EIntOp : forall (M5:M) (L5:L) (H5:H) (Clobber5:list emem) (C5:list e) (e1 e2 v_5:e) (E_5:E) (v1:e) (E1:E) (v2:e) (E2:E)
      (prod1value: eval M5 L5 H5 Clobber5 C5 e1 v1 E1)
      (prod2value: eval M5 L5 H5 Clobber5 C5 e2 v2 E2),
      is_L_of_L L5 ->
@@ -1351,7 +1409,7 @@ is_L_of_L L5 ->
      is_v_of_e v1 ->
      is_v_of_e v2 ->
      eval M5 L5 H5 Clobber5 C5 (E_IntOp e1 e2) v_5 E_5
- | EComp : forall (M5:M) (L5:L) (H5:H) (Clobber5:Clobber) (C5:list e) (e1 e2 v_5:e) (E_5:E) (v1:e) (E1:E) (v2:e) (E2:E)
+ | EComp : forall (M5:M) (L5:L) (H5:H) (Clobber5:list emem) (C5:list e) (e1 e2 v_5:e) (E_5:E) (v1:e) (E1:E) (v2:e) (E2:E)
      (prod1value: eval M5 L5 H5 Clobber5 C5 e1 v1 E1)
      (prod2value: eval M5 L5 H5 Clobber5 C5 e2 v2 E2),
      is_L_of_L L5 ->
@@ -1361,7 +1419,7 @@ is_L_of_L L5 ->
      is_v_of_e v1 ->
      is_v_of_e v2 ->
      eval M5 L5 H5 Clobber5 C5 (E_Comp e1 e2) v_5 E_5
- | ELet : forall (M5:M) (L5:L) (H5:H) (Clobber5:Clobber) (C5:list e) (id5:id) (T5:T) (e1 e2 v_5:e) (E_5 E1:E) (v2:e) (E2:E) (L':L) (v1:e)
+ | ELet : forall (M5:M) (L5:L) (H5:H) (Clobber5:list emem) (C5:list e) (id5:id) (T5:T) (e1 e2 v_5:e) (E_5 E1:E) (v2:e) (E2:E) (L':L) (v1:e)
      (prod1value: eval M5 L5 H5 Clobber5 C5 e1 v1 E1)
      (prod2value: eval M5 L5 H5 Clobber5 C5 e2 v2 E2),
      is_L_of_L L5 ->
@@ -1374,7 +1432,7 @@ is_L_of_L L5 ->
      is_v_of_e v1 ->
        L'   =   (L_LRepl L5 v1 id5)   ->
      eval M5 L5 H5 Clobber5 C5 (E_Let id5 T5 e1 e2) v_5 E_5
- | EIfTrue : forall (M5:M) (L5:L) (H5:H) (Clobber5:Clobber) (C5:list e) (e1 e2 e3 v5:e) (E_5 E1:E)
+ | EIfTrue : forall (M5:M) (L5:L) (H5:H) (Clobber5:list emem) (C5:list e) (e1 e2 e3 v5:e) (E_5 E1:E)
      (prod1value: eval M5 L5 H5 Clobber5 C5 e1 (E_Base1 bv_True) E1)
      (prod1value: eval M5 L5 H5 Clobber5 C5 e2 v5 E1),
      is_L_of_L L5 ->
@@ -1383,7 +1441,7 @@ is_L_of_L L5 ->
      is_e_of_e e3 ->
      is_v_of_e v5 ->
      eval M5 L5 H5 Clobber5 C5 (E_If e1 e2 e3) v5 E_5
- | EIfFalse : forall (M5:M) (L5:L) (H5:H) (Clobber5:Clobber) (C5:list e) (e1 e2 e3 v5:e) (E_5 E1 E2:E)
+ | EIfFalse : forall (M5:M) (L5:L) (H5:H) (Clobber5:list emem) (C5:list e) (e1 e2 e3 v5:e) (E_5 E1 E2:E)
      (prod1value: eval M5 L5 H5 Clobber5 C5 e1 (E_Base1 bv_False) E1)
      (prod2value: eval M5 L5 H5 Clobber5 C5 e3 v5 E2),
      is_L_of_L L5 ->
@@ -1392,52 +1450,52 @@ is_L_of_L L5 ->
      is_e_of_e e3 ->
      is_v_of_e v5 ->
      eval M5 L5 H5 Clobber5 C5 (E_If e1 e2 e3) v5 E_5
- | EFuncDef : forall (e_list:list_e) (r_list:list_r) (M5:M) (L5:L) (H5:H) (Clobber5:Clobber) (C5:list e) (id5:id) (v5:e) (E5:E) (L':L),
+ | EFuncDef : forall (e_list:list_e) (r_list:list_r) (M5:M) (L5:L) (H5:H) (Clobber5:list emem) (C5:list e) (id5:id) (v5:e) (E5:E) (L':L),
      is_L_of_L L5 ->
      is_v_of_e v5 ->
      is_L_of_L L' ->
      (Forall (fun (e_:e) => is_e_of_e e_) (unmake_list_e e_list)) ->
        L'   =   (L_LRepl L5 (E_FuncCall id5 r_list e_list) id5)   ->
      eval M5 L5 H5 Clobber5 C5 (E_FuncDef id5 r_list e_list) v5 E5
- | EFuncDefList : forall (id_rr_ee_list:list_id_rr_ee) (M5:M) (L5:L) (H5:H) (Clobber5:Clobber) (C5:list e) (v5:e) (E5:E),
+ | EFuncDefList : forall (id_rr_ee_list:list_id_rr_ee) (M5:M) (L5:L) (H5:H) (Clobber5:list emem) (C5:list e) (v5:e) (E5:E),
      is_L_of_L L5 ->
      is_v_of_e v5 ->
      (Forall (fun (tmp_:(id*rr*ee)) => match tmp_ with (id_,rr_,ee_) => is_ee_of_ee ee_ end) (unmake_list_id_rr_ee id_rr_ee_list)) ->
      eval M5 L5 H5 Clobber5 C5 (E_FuncDefList id_rr_ee_list) v5 E5
- | ETypedExpr : forall (M5:M) (L5:L) (H5:H) (Clobber5:Clobber) (C5:list e) (e5:e) (T5:T) (v5:e) (E5:E),
+ | ETypedExpr : forall (M5:M) (L5:L) (H5:H) (Clobber5:list emem) (C5:list e) (e5:e) (T5:T) (v5:e) (E5:E),
      is_L_of_L L5 ->
      is_e_of_e e5 ->
      is_v_of_e v5 ->
      eval M5 L5 H5 Clobber5 C5 e5 v5 E5 ->
      eval M5 L5 H5 Clobber5 C5 (E_TypedExpr e5 T5) v5 E5
- | EPlace : forall (M5:M) (L5:L) (H5:H) (Clobber5:Clobber) (C5:list e) (E5:E),
+ | EPlace : forall (M5:M) (L5:L) (H5:H) (Clobber5:list emem) (C5:list e) (E5:E),
      is_L_of_L L5 ->
      eval M5 L5 H5 Clobber5 C5 E_PlaceHolder E_PlaceHolder E5
- | Ebv : forall (M5:M) (L5:L) (H5:H) (Clobber5:Clobber) (C5:list e) (bv5:bv) (E5:E),
+ | Ebv : forall (M5:M) (L5:L) (H5:H) (Clobber5:list emem) (C5:list e) (bv5:bv) (E5:E),
      is_L_of_L L5 ->
      eval M5 L5 H5 Clobber5 C5 (E_Base1 bv5) (E_Base1 bv5) E5
- | Eiv : forall (M5:M) (L5:L) (H5:H) (Clobber5:Clobber) (C5:list e) (iv5:iv) (E5:E),
+ | Eiv : forall (M5:M) (L5:L) (H5:H) (Clobber5:list emem) (C5:list e) (iv5:iv) (E5:E),
      is_L_of_L L5 ->
      eval M5 L5 H5 Clobber5 C5 (E_Base2 iv5) (E_Base2 iv5) E5
- | ETuple : forall (M5:M) (L5:L) (H5:H) (Clobber5:Clobber) (C5:list e) (v1 v2:e) (E5:E),
+ | ETuple : forall (M5:M) (L5:L) (H5:H) (Clobber5:list emem) (C5:list e) (v1 v2:e) (E5:E),
      is_L_of_L L5 ->
      is_v_of_e v1 ->
      is_v_of_e v2 ->
      eval M5 L5 H5 Clobber5 C5 (E_Tuple v1 v2) (E_Tuple v1 v2) E5
- | ENullLoc : forall (M5:M) (L5:L) (H5:H) (Clobber5:Clobber) (C5:list e) (E5:E),
+ | ENullLoc : forall (M5:M) (L5:L) (H5:H) (Clobber5:list emem) (C5:list e) (E5:E),
      is_L_of_L L5 ->
      eval M5 L5 H5 Clobber5 C5 E_NullLoc E_NullLoc E5
- | EMemoryLoc : forall (M5:M) (L5:L) (H5:H) (Clobber5:Clobber) (C5:list e) (l5:l) (E5:E),
+ | EMemoryLoc : forall (M5:M) (L5:L) (H5:H) (Clobber5:list emem) (C5:list e) (l5:l) (E5:E),
      is_L_of_L L5 ->
      eval M5 L5 H5 Clobber5 C5 (E_MemoryLoc l5) (E_MemoryLoc l5) E5
- | ERegRelInst : forall (rho_list:list_rho) (M5:M) (L5:L) (H5:H) (Clobber5:Clobber) (C5:list e) (v5:e) (E5:E),
+ | ERegRelInst : forall (rho_list:list_rho) (M5:M) (L5:L) (H5:H) (Clobber5:list emem) (C5:list e) (v5:e) (E5:E),
      is_L_of_L L5 ->
      is_v_of_e v5 ->
      eval M5 L5 H5 Clobber5 C5 (E_RegRelInst rho_list v5) (E_RegRelInst rho_list v5) E5
- | EHeapVal : forall (M5:M) (L5:L) (H5:H) (Clobber5:Clobber) (C5:list e) (E5:E),
+ | EHeapVal : forall (M5:M) (L5:L) (H5:H) (Clobber5:list emem) (C5:list e) (E5:E),
      is_L_of_L L5 ->
      eval M5 L5 H5 Clobber5 C5 (E_HeapVal H5) (E_HeapVal H5) E5
- | EKthing : forall (M5:M) (L5:L) (H5:H) (Clobber5:Clobber) (C5:list e) (K5:K) (E5:E),
+ | EKthing : forall (M5:M) (L5:L) (H5:H) (Clobber5:list emem) (C5:list e) (K5:K) (E5:E),
      is_L_of_L L5 ->
      eval M5 L5 H5 Clobber5 C5 (E_Kthing K5) (E_Kthing K5) E5.
 Notation "G , P , O |- e : T ":= (typing G P O e T) (no associativity, at level 99). 
@@ -1445,7 +1503,7 @@ Notation "M , L , H , S , C |- e |-> v , E" := (eval M L H S C e v E) (no associ
 
 (* need theorem to prove that all top level e there is a typing rule *)
 
-Theorem preservation : forall (e5:e) (t:T) (E:E) (M:M) (L:L) (H:H) (S:Clobber) (C:list e) (T:T),
+Theorem preservation : forall (e5:e) (t:T) (E:E) (M:M) (L:L) (H:H) (S:list emem) (C:list e) (T:T),
     exists v,
       eval M L H S C e5 v E ->
       typing G_EmptyContext P_EmptyPriv O_EmptyConstraint e5 T  ->
@@ -1466,7 +1524,7 @@ Admitted.
 
 
 Theorem paper1 :
- forall (e5:e) (t:T) (M:M) (H:H) (S:Clobber) (C:C) (T1 T2:T)  G P O,
+ forall (e5:e) (t:T) (M:M) (H:H) (S:list emem) (C:C) (T1 T2:T)  G P O,
      typing G P O e5 T1 /\ eval M L H S C e5 v E /\ map_consist M O /\ local_val_consit L H /\ store_consist S H ->
      result_consist v H M T  /\ memory_trace_consist E H /\ trace_has_privs E P
 
@@ -1488,7 +1546,7 @@ forall (l: list (e * P)) M L H S,
        valid_interleaving
 
 Theorem paper5 :
- forall (e5:e) (t:T) (M:M) (H:H) (S:Clobber) (C:C) (T1 T2:T)  G P O,
+ forall (e5:e) (t:T) (M:M) (H:H) (S:list emem) (C:C) (T1 T2:T)  G P O,
      (types1: typing G P O e1 T1)
      (types2: typing G P O e2 T1)
      (privsmatch: pound_M P1  P2)
@@ -1504,7 +1562,7 @@ E :M Φ ⇔ ∀ ∈ E.
 ( = reduceid(l, c, v, t) ⇒ ∃r, l ∈ M(r) ∧ reducesid(r) ∈ Φ)
 *)
 
-Theorem progress : forall (e5:e) (t:T) (M:M) (H:H) (S:Clobber) (C:list e) (T1 T2:T),
+Theorem progress : forall (e5:e) (t:T) (M:M) (H:H) (S:list emem) (C:list e) (T1 T2:T),
      exists E L v,
      typing G_EmptyContext P_EmptyPriv O_EmptyConstraint e5 T1  ->
        typing G_EmptyContext P_EmptyPriv O_EmptyConstraint v T2  ->
@@ -1577,7 +1635,7 @@ Proof.
     intros.
     inversion H2.
   - (* Read *)
-    exists ([] ++ [em_ReadE (E_MemoryLoc ML_NilLoc) EX_Nil (E_HeapVal (H_Hl H0 ML_NilLoc))  E_Zero]). 
+    exists ([] ++ [em_ReadE (E_MemoryLoc ML_NilLoc) priv_excl (E_HeapVal (H_Hl H0 ML_NilLoc))  E_Zero]). 
 
     exists L_Nil. 
     repeat eexists.
@@ -1613,9 +1671,35 @@ Proof.
     exists L_Nil.
     repeat eexists.
     intros.
-    apply EWrite with (E1:=[]) (Clobber':=S) (v5:=(E_MemoryLoc ML_NilLoc)) (E2:=[]).
+    apply EWrite with (E1:=[]) (Clobber':=[]) (v5:=(E_MemoryLoc ML_NilLoc)) (E2:=[]).
     inversion H2.
     inversion H2.
+    simpl.
+    intros.
+    induction S.
+    simpl.
+    repeat (split; auto).
+    intros.
+    induction (fold_right (fun a b : list emem => a ++ b) [] l0).
+    reflexivity.
+    simpl.
+    destruct a;inversion IHl1; reflexivity.
+    simpl.
+    repeat (split; auto).
+    intros.
+    induction (fold_right (fun a0 b : list emem => a0 ++ b) [] l0).
+    reflexivity.
+
+    destruct a0; simpl; assumption.
+    ;inversion IHl1; reflexivity.
+
+    reflexivity.
+    reflexivity.
+    reflexivity.
+    ; reflexivity.
+    rewrite <- IHl1.
+    j
+    apply IHl0.
     reflexivity.
     inversion H2.
     inversion H2.
